tests/c-test/main_c_proof.v
@@ -18,6 +18,40 @@ Lemma can_get_element {T} :
     exists (v : T) (i : nat), Z.of_nat i = x4 /\ nth_error x3 i = Some v.
 Proof. Admitted.
 
+Lemma skipn_allZ : forall {T} (ls : list T) x,
+    x >= Z.of_nat (Datatypes.length ls) ->
+    skipn (Z.to_nat x) ls = nil.
+Proof.
+  induction ls; simpl; intros.
+  { destruct (Z.to_nat x); auto. }
+  { destruct (Z.to_nat x) eqn:?.
+    { simpl. exfalso. destruct x; simpl in *; try lia. }
+    erewrite <- IHls.
+    simpl. instantiate (1 := x-1).
+    f_equal.
+    rewrite (Znat.Z2Nat.inj_sub x 1); simpl.
+    rewrite Heqn. lia. lia. lia. }
+Qed.
+
+Lemma skipn_to_nat_of_nat:
+  forall (x3 : list string) (x4 : Z),
+    x4 < Z.of_nat (Datatypes.length x3) ->
+    forall x6 : nat,
+      Z.of_nat x6 = x4 ->
+      match x3 with
+      | nil => nil
+      | _ :: l0 => skipn (Z.to_nat x4) l0
+      end = skipn (Z.to_nat (Z.of_nat x6 + 1)) x3.
+Proof.
+  intros x3 x4 l x6 H2.
+  generalize (Znat.Nat2Z.inj_add x6 1); simpl; intros.
+  rewrite <- H; clear H.
+  subst.
+  cutrewrite (Z.to_nat (Z.of_nat (x6 + 1)) = S (Z.to_nat (Z.of_nat x6))).
+  reflexivity.
+  rewrite <- Znat.Z2Nat.inj_succ; lia.
+Qed.
+
 (* soundness of the specification *)
 Theorem main_cpp_sound : forall (resolve : genv),
     denoteModule main_c.module |-- spec resolve.
@@ -40,11 +74,12 @@ Proof.
         (ti_cglob' (resolve:=resolve) "_Z6putstr" putstr_spec **
          tlocal x1 (Tint None true) "argc" x **
          tlocal x1 (Tpointer (Qmut (Tpointer (Qmut T_char)))) "argv" x0) **
-         (Forall res : val, [| res = 0 |] ** args_array x0 x3 -* x2 res) **
+         (Forall res : val, [| res = 0 |] ** args_array x0 x3 ** @trace PutStr (Ret tt) -* x2 res) **
          args_array x0 x3 **
          Exists i,
            [| 0 <= i <= Z.of_nat (Datatypes.length x3) |] **
-           tlocal x1 T_int "i" i).
+           tlocal x1 T_int "i" i **
+           trace (printEach (skipn (Z.to_nat i) x3))).
     { work. }
     eapply wp_for.
     simplifying.
@@ -58,7 +93,7 @@ Proof.
       unfold args_array.
       assert (exists v, exists i, Z.of_nat i = x4 /\ nth_error x3 i = Some v).
       { eapply can_get_element; eauto. }
-      destruct H1 as [ ? [ ? [ ? ? ] ] ].
+      destruct H2 as [ ? [ ? [ ? ? ] ] ].
       rewrite tarray_cell; eauto with size_of.
       rewrite <- wp_lhs_subscript.
       simplifying.
@@ -67,22 +102,35 @@ Proof.
       simplifying.
       work.
       { subst. work. }
-      simplifying. simpl.
+      simplifying.
+      instantiate (1 := (x5, printEach (skipn (S (Z.to_nat x4)) x3))).
+      simpl.
       unfold tlocal.
       lift_ex_l.
       perm_left ltac:(idtac; eapply (Lemmas.learn_bounds x4); simpl; intros).
       work.
-      instantiate (1:=Vint (x4 + 1)).
-      eapply provable_star.
-      { eapply eval_add. reflexivity.
-        eapply has_type_int_any. }
-      work.
-      rewrite tarray_cell with (ms:=x3); eauto with size_of.
-      work. }
+      cutrewrite (skipn (Z.to_nat x4) x3 = x5 :: skipn (S (Z.to_nat x4)) x3).
+      { simpl. work.
+        simplifying.
+        work.
+        rewrite tarray_cell with (ms :=x3); eauto with size_of.
+        work.
+        erewrite skipn_to_nat_of_nat; eauto. reflexivity. }
+      { simpl. subst.
+        rewrite Znat.Nat2Z.id.
+        clear - H3.
+        generalize dependent x6.
+        induction x3.
+        { destruct x6; simpl in *; congruence. }
+        { intros.
+          destruct x6; simpl in *.
+          inversion H3; clear H3; subst; auto.
+          eauto. } } }
     { simpl.
       unfold Sskip.
       simplifying.
       work.
+      rewrite skipn_allZ; eauto.
       done_proof. } }
 
   finish_module.
